generalised NQueens to BOARD_SIZE

plugins/vdm2isa/isa/NQueens.thy
@@ -1,49 +1,100 @@
 theory NQueens
-imports VDMToolkit
+imports VDMToolkit "HOL-Library.Multiset_Order"
 begin
 
-type_synonym Pos = "VDMNat \<times> VDMNat" 
+abbreviation
+  BOARD_SIZE :: \<open>VDMNat1\<close>
+  where
+  "BOARD_SIZE \<equiv> 8"
+
+abbreviation
+  MAX_QUEENS :: \<open>VDMNat1\<close>
+  where
+  "MAX_QUEENS \<equiv> BOARD_SIZE + 1"
+
+type_synonym Queens = "VDMNat1" 
 
 definition 
-  inv_Pos :: "Pos \<Rightarrow> \<bool>"
+  inv_Queens :: \<open>VDMNat1 \<Rightarrow> \<bool>\<close>
   where
-  "inv_Pos p \<equiv> inv_VDMNat (fst p) \<and> inv_VDMNat (snd p)"
+  \<open>inv_Queens q \<equiv> inv_VDMNat1 q \<and> q \<le> MAX_QUEENS\<close>
 
-type_synonym Board = "Pos VDMSet"
+type_synonym Pos = "VDMNat" 
+
+definition 
+  inv_Pos :: \<open>VDMNat \<Rightarrow> \<bool>\<close>
+  where
+  "inv_Pos p \<equiv> inv_VDMNat p \<and> p < BOARD_SIZE"
+
+lemmas inv_Pos_defs = inv_Pos_def inv_VDMNat_def
+
+type_synonym Coord = "Pos \<times> Pos" 
+
+definition 
+  inv_Coord :: "Coord \<Rightarrow> \<bool>"
+  where
+  "inv_Coord p \<equiv> let (r,c) = p in inv_Pos r \<and> inv_Pos c"
+
+lemmas inv_Coord_defs = inv_Coord_def inv_Pos_defs 
+
+type_synonym Board = "Coord VDMSet"
 
 definition 
   inv_Board :: "Board \<Rightarrow> \<bool>"
   where
-  "inv_Board b \<equiv> inv_VDMSet' inv_Pos b"
+  "inv_Board b \<equiv> inv_VDMSet' inv_Coord b"
+
+lemmas inv_Board_defs = inv_VDMSet'_defs inv_Coord_defs
+
+definition
+  pre_allowed :: \<open>VDMNat \<Rightarrow> VDMNat \<Rightarrow> Board \<Rightarrow> \<bool>\<close>
+  where 
+  \<open>pre_allowed r c b \<equiv> inv_VDMNat r \<and> inv_VDMNat c \<and> inv_Board b\<close>
+
+lemmas pre_allowed_defs = inv_VDMNat_def inv_Board_defs
+(*
+definition 
+  post_allowed :: \<open>VDMNat \<Rightarrow> VDMNat \<Rightarrow> Board \<Rightarrow> \<bool> \<Rightarrow> \<bool>\<close>
+  where 
+ \<open>post_allowed r c b RESULT \<equiv> 
+    pre_allowed r c b \<longrightarrow> RESULT \<longrightarrow> post_vdm_abs (r - r') (vdm_abs (r - r')) \<close>
+*)
 
 definition 
-  allowed :: \<open>VDMNat \<Rightarrow> VDMNat \<Rightarrow> Board \<Rightarrow> \<bool>\<close>
+  allowed :: \<open>Pos \<Rightarrow> Pos \<Rightarrow> Board \<Rightarrow> \<bool>\<close>
   where
   \<open>allowed r c board \<equiv> 
       (r, c) \<in> board \<and>
       \<not> (\<exists> b \<in> board . let (r',c') = b in r = r' \<or> c = c' \<or> vdm_abs (r - r') = vdm_abs (c - c'))
   \<close>
 
-definition 
-  pre_solve :: \<open>Board \<Rightarrow> VDMNat1 \<Rightarrow> \<bool>\<close>
-  where
-\<open>pre_solve board Q \<equiv> inv_Board board \<and> inv_VDMNat1 Q\<close>
+lemmas allowed_defs = allowed_def vdm_abs_def
 
 definition 
-  pre_trys :: \<open>Pos VDMSet \<Rightarrow> Board \<Rightarrow> VDMNat1 \<Rightarrow> \<bool>\<close>
+  pre_solve :: \<open>Board \<Rightarrow> Queens \<Rightarrow> \<bool>\<close>
   where
-\<open>pre_trys possible board Q \<equiv> inv_VDMSet' inv_Pos possible \<and> inv_Board board \<and> inv_VDMNat1 Q\<close>
+\<open>pre_solve board Q \<equiv> inv_Board board \<and> inv_Queens Q\<close>
 
+definition 
+  pre_trys :: \<open>Coord VDMSet \<Rightarrow> Board \<Rightarrow> VDMNat1 \<Rightarrow> \<bool>\<close>
+  where
+\<open>pre_trys possible board Q \<equiv> inv_VDMSet' inv_Coord possible \<and> inv_Board board \<and> inv_Queens Q\<close>
+
+lemmas pre_solve_defs = pre_solve_def inv_Board_def inv_VDMNat1_def 
+lemmas pre_trys_defs  = pre_trys_def inv_VDMSet'_def inv_Coord_defs inv_Board_defs inv_VDMNat1_def
+declare pre_solve_defs []
+declare pre_trys_defs []
+declare allowed_defs []
 function (domintros)
-  solve :: \<open>Board \<Rightarrow> VDMNat1 \<Rightarrow> Board option\<close> and
-  trys  :: \<open>Pos VDMSet \<Rightarrow> Board \<Rightarrow> VDMNat1 \<Rightarrow> Board option\<close>
+  solve :: \<open>Board \<Rightarrow> Queens \<Rightarrow> Board option\<close> and
+  trys  :: \<open>Coord VDMSet \<Rightarrow> Board \<Rightarrow> Queens \<Rightarrow> Board option\<close>
   where 
   \<open>solve board Q = 
       (if pre_solve board Q then 
-          (if Q = 9 then 
+          (if Q = MAX_QUEENS then 
             Some board 
           else 
-            (let possible = { (r, c) | r c . r \<in> {(0::VDMNat)..7} \<and> c \<in> {0..7} \<and> (allowed r c board) } in
+            (let possible = { (r, c) | r c . r \<in> {(0::VDMNat)..BOARD_SIZE-1} \<and> c \<in> {0..BOARD_SIZE-1} \<and> (allowed r c board) } in
                 (trys possible board Q))
           )
        else 
@@ -51,8 +102,11 @@ function (domintros)
   \<close>
 | \<open>trys possible board Q = 
     (if pre_trys possible board Q then 
-       let p = (\<some> x . x \<in> possible) in 
-          let solution = solve (board \<union> {p}) (Q+1) in 
+       if possible = {} then
+          None 
+       else 
+          let p = (\<some> x . x \<in> possible);
+              solution = solve (board \<union> {p}) (Q+1) in 
             if solution = None then 
               (trys (possible - {p}) board Q)
             else
@@ -62,7 +116,24 @@ function (domintros)
     )
   \<close>
   by (pat_completeness, auto)
+
+lemma l_board_size: \<open>inv_Board board \<Longrightarrow> vdm_card board \<le> 64\<close> oops
+
 termination 
+  apply (relation \<open>
+      measure (\<lambda> x . 
+                case x of 
+                    Inl (board, Q) \<Rightarrow> if Q = MAX_QUEENS then 0 else nat ((BOARD_SIZE*BOARD_SIZE) - (vdm_card board))
+                  | Inr (possible, board, Q) \<Rightarrow> if possible = {} then 0 else nat (Q+1) )\<close>)
+     apply simp
+    apply (simp add: pre_solve_def)
+    apply (intro allI conjI impI)
+      apply (erule allE[of _ "0::Pos"])+
+  apply simp unfolding allowed_def vdm_abs_def apply simp 
+  find_theorems "_ = (_::'a set)" elim
+  apply (elim equalityE)
+  apply (simp add: set_of_pred_def)
+  find_theorems "_ = _Collect _"
   oops
 
 definition
